specs/lib/Spec.Lib.IntBuf.LoadStore.fsti
@@ -10,7 +10,7 @@ open Spec.Lib.IntBuf
 
 inline_for_extraction
 val uints_from_bytes_le:
-  #t:inttype -> #len:size_nat{len `op_Multiply` numbytes t <= max_size_t} ->
+  #t:m_inttype -> #len:size_nat{len `op_Multiply` numbytes t <= max_size_t} ->
   o:lbuffer (uint_t t) (len) ->
   i:lbuffer uint8 (len `op_Multiply` numbytes t) ->
   Stack unit
@@ -22,7 +22,7 @@ val uints_from_bytes_le:
 
 inline_for_extraction
 val uints_from_bytes_be:
-  #t:inttype -> #len:size_nat{len `op_Multiply` numbytes t <= max_size_t} ->
+  #t:m_inttype -> #len:size_nat{len `op_Multiply` numbytes t <= max_size_t} ->
   o:lbuffer (uint_t t) (len) ->
   i:lbuffer uint8 (len `op_Multiply` numbytes t) ->
   Stack unit
@@ -32,28 +32,32 @@ val uints_from_bytes_be:
 			      as_lseq o h1 ==
 			      (LSeq.uints_from_bytes_be #t #(len) (as_lseq i h0) )))
 
-inline_for_extraction
-val uint32s_from_bytes_le:
-  #len:size_nat{len `op_Multiply` 4 <= max_size_t} ->
-  clen:size_t{size_v clen == len} ->
-  o:lbuffer uint32 len ->
-  i:lbuffer uint8 (len `op_Multiply` 4) ->
-  Stack unit
-	(requires (fun h0 -> live h0 o /\ live h0 i /\ disjoint o i))
-	(ensures (fun h0 _ h1 -> preserves_live h0 h1 /\
-			      modifies1 o h0 h1 /\
-			      as_lseq o h1 ==
-			      (LSeq.uints_from_bytes_le #U32 #len (as_lseq i h0) )))
 
 inline_for_extraction
-val uint32s_to_bytes_le:
-  #len:size_nat{len `op_Multiply` 4 <= max_size_t} ->
-  clen:size_t{size_v clen == len} ->
-  o:lbuffer uint8 (len `op_Multiply` 4) ->
-  i:lbuffer uint32 len ->
+val uints_to_bytes_le:
+  #t:m_inttype -> #len:size_nat{len `op_Multiply` numbytes t <= max_size_t} ->
+  o:lbuffer uint8 (len `op_Multiply` numbytes t) ->
+  i:lbuffer (uint_t t) (len) ->
   Stack unit
 	(requires (fun h0 -> live h0 o /\ live h0 i))
 	(ensures (fun h0 _ h1 -> preserves_live h0 h1 /\
 			      modifies1 o h0 h1 /\
 			      as_lseq o h1 ==
-			      (LSeq.uints_to_bytes_le #U32 #len (as_lseq i h0) )))
+			      (LSeq.uints_to_bytes_le #t #(len) (as_lseq i h0) )))
+
+inline_for_extraction
+val uints_to_bytes_be:
+  #t:m_inttype -> #len:size_nat{len `op_Multiply` numbytes t <= max_size_t} ->
+  o:lbuffer uint8 (len `op_Multiply` numbytes t) ->
+  i:lbuffer (uint_t t) (len) ->
+  Stack unit
+	(requires (fun h0 -> live h0 o /\ live h0 i))
+	(ensures (fun h0 _ h1 -> preserves_live h0 h1 /\
+			      modifies1 o h0 h1 /\
+			      as_lseq o h1 ==
+			      (LSeq.uints_to_bytes_be #t #(len) (as_lseq i h0) )))
+
+inline_for_extraction
+let uint32s_to_bytes_le = uints_to_bytes_le #U32
+inline_for_extraction
+let uint32s_from_bytes_le = uints_from_bytes_le #U32
